@prefix cc: <http://creativecommons.org/ns#> .
@prefix dc: <http://purl.org/dc/terms/> .
@prefix hydra: <http://www.w3.org/ns/hydra/core#> .
@prefix owl: <http://www.w3.org/2002/07/owl#> .
@prefix rdf: <http://www.w3.org/1999/02/22-rdf-syntax-ns#> .
@prefix rdfs: <http://www.w3.org/2000/01/rdf-schema#> .
@prefix schema: <http://schema.org/> .
@prefix vann: <http://purl.org/vocab/vann/> .
@prefix vs: <http://www.w3.org/2003/06/sw-vocab-status/ns#> .
@prefix xsd: <http://www.w3.org/2001/XMLSchema#> .

hydra:Class a rdfs:Class,
        hydra:Resource ;
    rdfs:label "Hydra Class" ;
    rdfs:comment "The class of Hydra classes." ;
    rdfs:isDefinedBy <http://www.w3.org/ns/hydra/core> ;
    rdfs:subClassOf rdfs:Class ;
    vs:term_status "testing" .

hydra:HeaderSpecification a rdfs:Class ;
    rdfs:label "Header specification" ;
    rdfs:comment "Specifies a possible either expected or returned header values" ;
    rdfs:isDefinedBy <http://www.w3.org/ns/hydra/core> ;
    rdfs:subClassOf hydra:Resource ;
    vs:term_status "testing" .

hydra:BasicRepresentation a hydra:VariableRepresentation ;
    rdfs:label "BasicRepresentation" ;
    rdfs:comment "A representation that serializes just the lexical form of a variable value, but omits language and type information." ;
    rdfs:isDefinedBy <http://www.w3.org/ns/hydra/core> ;
    vs:term_status "testing" .

hydra:Error a hydra:Class ;
    rdfs:label "Error" ;
    rdfs:comment "A runtime error, used to report information beyond the returned status code." ;
    rdfs:isDefinedBy <http://www.w3.org/ns/hydra/core> ;
    rdfs:subClassOf hydra:Status ;
    vs:term_status "testing" .

hydra:ExplicitRepresentation a hydra:VariableRepresentation ;
    rdfs:label "ExplicitRepresentation" ;
    rdfs:comment "A representation that serializes a variable value including its language and type information and thus differentiating between IRIs and literals." ;
    rdfs:isDefinedBy <http://www.w3.org/ns/hydra/core> ;
    vs:term_status "testing" .

hydra:LinkContext a hydra:BaseUriSource ;
    rdfs:label "Link context" ;
    rdfs:comment "States that the link's context IRI, as defined in RFC 5988, should be used as the base Uri" ;
    rdfs:isDefinedBy <http://www.w3.org/ns/hydra/core> ;
    vs:term_status "testing" .

hydra:PartialCollectionView a hydra:Class ;
    rdfs:label "PartialCollectionView" ;
    rdfs:comment "A PartialCollectionView describes a partial view of a Collection. Multiple PartialCollectionViews can be connected with the the next/previous properties to allow a client to retrieve all members of the collection." ;
    rdfs:isDefinedBy <http://www.w3.org/ns/hydra/core> ;
    rdfs:subClassOf hydra:Resource ;
    vs:term_status "testing" .

hydra:Rfc3986 a hydra:BaseUriSource ;
    rdfs:label "RFC 3986 based" ;
    rdfs:comment "States that the base Uri should be established using RFC 3986 reference resolution algorithm specified in section 5." ;
    rdfs:isDefinedBy <http://www.w3.org/ns/hydra/core> ;
    vs:term_status "testing" .

hydra:apiDocumentation a hydra:Link ;
    rdfs:label "apiDocumentation" ;
    rdfs:comment "A link to the API documentation" ;
    rdfs:domain hydra:Resource ;
    rdfs:isDefinedBy <http://www.w3.org/ns/hydra/core> ;
    rdfs:range hydra:ApiDocumentation ;
    vs:term_status "testing" .

hydra:closedSet a rdf:Property ;
    rdfs:label "closed set" ;
    rdfs:comment "Determines whether the provided set of header values is closed or not." ;
    rdfs:domain hydra:HeaderSpecification ;
    rdfs:isDefinedBy <http://www.w3.org/ns/hydra/core> ;
    rdfs:range xsd:boolean ;
    vs:term_status "testing" .

hydra:collection a hydra:Link ;
    rdfs:label "collection" ;
    rdfs:comment "Collections somehow related to this resource." ;
    rdfs:isDefinedBy <http://www.w3.org/ns/hydra/core> ;
    rdfs:range hydra:Collection ;
    vs:term_status "testing" .

hydra:description a rdf:Property ;
    rdfs:label "description" ;
    schema:domainIncludes hydra:ApiDocumentation,
        hydra:Class,
        hydra:Link,
        hydra:Operation,
        hydra:Status,
        hydra:SupportedProperty,
        hydra:TemplatedLink ;
    rdfs:comment "A description." ;
    rdfs:isDefinedBy <http://www.w3.org/ns/hydra/core> ;
    rdfs:range xsd:string ;
    rdfs:subPropertyOf rdfs:comment ;
    vs:term_status "testing" .

hydra:entrypoint a hydra:Link ;
    rdfs:label "entrypoint" ;
    rdfs:comment "A link to main entry point of the Web API" ;
    rdfs:domain hydra:ApiDocumentation ;
    rdfs:isDefinedBy <http://www.w3.org/ns/hydra/core> ;
    rdfs:range hydra:Resource ;
    vs:term_status "testing" .

hydra:expects a hydra:Link ;
    rdfs:label "expects" ;
    schema:rangeIncludes rdfs:Class,
        rdfs:Resource,
        hydra:Class,
        hydra:Resource ;
    rdfs:comment "The information expected by the Web API." ;
    rdfs:domain hydra:Operation ;
    rdfs:isDefinedBy <http://www.w3.org/ns/hydra/core> ;
    vs:term_status "testing" .

hydra:expectsHeader a rdf:Property ;
    rdfs:label "expects header" ;
    schema:rangeIncludes xsd:string,
        hydra:HeaderSpecification ;
    rdfs:comment "Specification of the header expected by the operation." ;
    rdfs:domain hydra:Operation ;
    rdfs:isDefinedBy <http://www.w3.org/ns/hydra/core> ;
    vs:term_status "testing" .

hydra:extension a rdf:Property ;
    rdfs:label "extension" ;
    rdfs:comment "Hint on what kind of extensions are in use." ;
    rdfs:domain hydra:ApiDocumentation ;
    rdfs:isDefinedBy <http://www.w3.org/ns/hydra/core> ;
    vs:term_status "testing" .

hydra:first a hydra:Link ;
    rdfs:label "first" ;
    rdfs:comment "The first resource of an interlinked set of resources." ;
    rdfs:domain hydra:Resource ;
    rdfs:isDefinedBy <http://www.w3.org/ns/hydra/core> ;
    rdfs:range hydra:Resource ;
    vs:term_status "testing" .

hydra:freetextQuery a rdf:Property ;
    rdfs:label "freetext query" ;
    rdfs:comment "A property representing a freetext query." ;
    rdfs:domain hydra:Resource ;
    rdfs:isDefinedBy <http://www.w3.org/ns/hydra/core> ;
    rdfs:range xsd:string ;
    vs:term_status "testing" .

hydra:headerName a rdf:Property ;
    rdfs:label "header name" ;
    rdfs:comment "Name of the header." ;
    rdfs:domain hydra:HeaderSpecification ;
    rdfs:isDefinedBy <http://www.w3.org/ns/hydra/core> ;
    rdfs:range xsd:string ;
    vs:term_status "testing" .

hydra:last a hydra:Link ;
    rdfs:label "last" ;
    rdfs:comment "The last resource of an interlinked set of resources." ;
    rdfs:domain hydra:Resource ;
    rdfs:isDefinedBy <http://www.w3.org/ns/hydra/core> ;
    rdfs:range hydra:Resource ;
    vs:term_status "testing" .

hydra:limit a rdf:Property ;
    rdfs:label "take" ;
    rdfs:comment "Instructs to limit set only to N elements." ;
    rdfs:isDefinedBy <http://www.w3.org/ns/hydra/core> ;
    rdfs:range xsd:nonNegativeInteger ;
    vs:term_status "testing" .

hydra:manages rdfs:label "manages" ;
    rdfs:comment "This predicate is left for compatibility purposes and hydra:memberAssertion should be used instead." ;
    rdfs:isDefinedBy <http://www.w3.org/ns/hydra/core> ;
    rdfs:subPropertyOf hydra:memberAssertion ;
    vs:term_status "archaic" .

hydra:mapping a rdf:Property ;
    rdfs:label "mapping" ;
    rdfs:comment "A variable-to-property mapping of the IRI template." ;
    rdfs:domain hydra:IriTemplate ;
    rdfs:isDefinedBy <http://www.w3.org/ns/hydra/core> ;
    rdfs:range hydra:IriTemplateMapping ;
    vs:term_status "testing" .

hydra:member a hydra:Link ;
    rdfs:label "member" ;
    rdfs:comment "A member of the collection" ;
    rdfs:domain hydra:Collection ;
    rdfs:isDefinedBy <http://www.w3.org/ns/hydra/core> ;
    vs:term_status "testing" .

hydra:method a rdf:Property ;
    rdfs:label "method" ;
    rdfs:comment "The HTTP method." ;
    rdfs:domain hydra:Operation ;
    rdfs:isDefinedBy <http://www.w3.org/ns/hydra/core> ;
    rdfs:range xsd:string ;
    vs:term_status "testing" .

hydra:next a hydra:Link ;
    rdfs:label "next" ;
    rdfs:comment "The resource following the current instance in an interlinked set of resources." ;
    rdfs:domain hydra:Resource ;
    rdfs:isDefinedBy <http://www.w3.org/ns/hydra/core> ;
    rdfs:range hydra:Resource ;
    vs:term_status "testing" .

hydra:object rdfs:label "object" ;
    rdfs:comment "The object." ;
    rdfs:isDefinedBy <http://www.w3.org/ns/hydra/core> ;
    vs:term_status "testing" .

hydra:offset a rdf:Property ;
    rdfs:label "skip" ;
    rdfs:comment "Instructs to skip N elements of the set." ;
    rdfs:isDefinedBy <http://www.w3.org/ns/hydra/core> ;
    rdfs:range xsd:nonNegativeInteger ;
    vs:term_status "testing" .

hydra:operation a hydra:Link ;
    rdfs:label "operation" ;
    rdfs:comment "An operation supported by the Hydra resource" ;
    rdfs:domain hydra:Resource ;
    rdfs:isDefinedBy <http://www.w3.org/ns/hydra/core> ;
    rdfs:range hydra:Operation ;
    vs:term_status "testing" .

hydra:pageIndex a rdf:Property ;
    rdfs:label "page index" ;
    rdfs:comment "Instructs to provide a specific page of the collection at a given index." ;
    rdfs:isDefinedBy <http://www.w3.org/ns/hydra/core> ;
    rdfs:range xsd:nonNegativeInteger ;
    rdfs:subPropertyOf hydra:pageReference ;
    vs:term_status "testing" .

hydra:possibleStatus a hydra:Link ;
    rdfs:label "possible status" ;
    schema:domainIncludes hydra:ApiDocumentation,
        hydra:Operation ;
    rdfs:comment "A status that might be returned by the Web API (other statuses should be expected and properly handled as well)" ;
    rdfs:isDefinedBy <http://www.w3.org/ns/hydra/core> ;
    rdfs:range hydra:Status ;
    vs:term_status "testing" .

hydra:possibleValue a rdf:Property ;
    rdfs:label "possible header value" ;
    rdfs:comment "Possible value of the header." ;
    rdfs:domain hydra:HeaderSpecification ;
    rdfs:isDefinedBy <http://www.w3.org/ns/hydra/core> ;
    rdfs:range xsd:string ;
    vs:term_status "testing" .

hydra:previous a hydra:Link ;
    rdfs:label "previous" ;
    rdfs:comment "The resource preceding the current instance in an interlinked set of resources." ;
    rdfs:domain hydra:Resource ;
    rdfs:isDefinedBy <http://www.w3.org/ns/hydra/core> ;
    rdfs:range hydra:Resource ;
    vs:term_status "testing" .

hydra:property a rdf:Property ;
    rdfs:label "property" ;
    schema:domainIncludes hydra:IriTemplateMapping,
        hydra:SupportedProperty ;
    rdfs:comment "A property" ;
    rdfs:isDefinedBy <http://www.w3.org/ns/hydra/core> ;
    rdfs:range rdf:Property ;
    vs:term_status "testing" .

hydra:readable a rdf:Property ;
    rdfs:label "readable" ;
    rdfs:comment "True if the client can retrieve the property's value, false otherwise." ;
    rdfs:domain hydra:SupportedProperty ;
    rdfs:isDefinedBy <http://www.w3.org/ns/hydra/core> ;
    rdfs:range xsd:boolean ;
    vs:term_status "testing" .

hydra:required a rdf:Property ;
    rdfs:label "required" ;
    schema:domainIncludes hydra:IriTemplateMapping,
        hydra:SupportedProperty ;
    rdfs:comment "True if the property is required, false otherwise." ;
    rdfs:isDefinedBy <http://www.w3.org/ns/hydra/core> ;
    rdfs:range xsd:boolean ;
    vs:term_status "testing" .

hydra:resolveRelativeUsing a rdf:Property ;
    rdfs:label "relative Uri resolution" ;
    rdfs:domain hydra:IriTemplate ;
    rdfs:isDefinedBy <http://www.w3.org/ns/hydra/core> ;
    rdfs:range hydra:BaseUriSource ;
    vs:term_status "testing" .

hydra:returns a hydra:Link ;
    rdfs:label "returns" ;
    schema:rangeIncludes rdfs:Class,
        rdfs:Resource,
        hydra:Class,
        hydra:Resource ;
    rdfs:comment "The information returned by the Web API on success" ;
    rdfs:domain hydra:Operation ;
    rdfs:isDefinedBy <http://www.w3.org/ns/hydra/core> ;
    vs:term_status "testing" .

hydra:returnsHeader a rdf:Property ;
    rdfs:label "returns header" ;
    schema:rangeIncludes xsd:string,
        hydra:HeaderSpecification ;
    rdfs:comment "Name of the header returned by the operation." ;
    rdfs:domain hydra:Operation ;
    rdfs:isDefinedBy <http://www.w3.org/ns/hydra/core> ;
    vs:term_status "testing" .

hydra:search a hydra:TemplatedLink ;
    rdfs:label "search" ;
    rdfs:comment "A IRI template that can be used to query a collection." ;
    rdfs:domain hydra:Resource ;
    rdfs:isDefinedBy <http://www.w3.org/ns/hydra/core> ;
    rdfs:range hydra:IriTemplate ;
    vs:term_status "testing" .

hydra:statusCode a rdf:Property ;
    rdfs:label "status code" ;
    rdfs:comment "The HTTP status code. Please note it may happen this value will be different to actual status code received." ;
    rdfs:domain hydra:Status ;
    rdfs:isDefinedBy <http://www.w3.org/ns/hydra/core> ;
    rdfs:range xsd:integer ;
    vs:term_status "testing" .

hydra:subject rdfs:label "subject" ;
    rdfs:comment "The subject." ;
    rdfs:isDefinedBy <http://www.w3.org/ns/hydra/core> ;
    vs:term_status "testing" .

hydra:supportedClass a hydra:Link ;
    rdfs:label "supported classes" ;
    rdfs:comment "A class known to be supported by the Web API" ;
    rdfs:domain hydra:ApiDocumentation ;
    rdfs:isDefinedBy <http://www.w3.org/ns/hydra/core> ;
    rdfs:range rdfs:Class ;
    vs:term_status "testing" .

hydra:supportedOperation a hydra:Link ;
    rdfs:label "supported operation" ;
    schema:domainIncludes rdfs:Class,
        hydra:Class,
        hydra:Link,
        hydra:SupportedProperty,
        hydra:TemplatedLink ;
    rdfs:comment "An operation supported by instances of the specific Hydra class, or the target of the Hydra link, or IRI template." ;
    rdfs:isDefinedBy <http://www.w3.org/ns/hydra/core> ;
    rdfs:range hydra:Operation ;
    vs:term_status "testing" .

hydra:supportedProperty a hydra:Link ;
    rdfs:label "supported properties" ;
    rdfs:comment "The properties known to be supported by a Hydra class" ;
    rdfs:domain rdfs:Class ;
    rdfs:isDefinedBy <http://www.w3.org/ns/hydra/core> ;
    rdfs:range hydra:SupportedProperty ;
    vs:term_status "testing" .

hydra:template a rdf:Property ;
    rdfs:label "template" ;
    rdfs:comment "A templated string with placeholders. The literal's datatype indicates the template syntax; if not specified, hydra:Rfc6570Template is assumed." ;
    rdfs:domain hydra:IriTemplate ;
    rdfs:isDefinedBy <http://www.w3.org/ns/hydra/core> ;
    rdfs:range hydra:Rfc6570Template ;
    rdfs:seeAlso hydra:Rfc6570Template ;
    vs:term_status "testing" .

hydra:title a rdf:Property ;
    rdfs:label "title" ;
    schema:domainIncludes hydra:ApiDocumentation,
        hydra:Class,
        hydra:Link,
        hydra:Operation,
        hydra:Status,
        hydra:SupportedProperty,
        hydra:TemplatedLink ;
    rdfs:comment "A title, often used along with a description." ;
    rdfs:isDefinedBy <http://www.w3.org/ns/hydra/core> ;
    rdfs:range xsd:string ;
    rdfs:subPropertyOf rdfs:label ;
    vs:term_status "testing" .

hydra:totalItems a rdf:Property ;
    rdfs:label "total items" ;
    rdfs:comment "The total number of items referenced by a collection." ;
    rdfs:domain hydra:Collection ;
    rdfs:isDefinedBy <http://www.w3.org/ns/hydra/core> ;
    rdfs:range xsd:integer ;
    vs:term_status "testing" .

hydra:variable a rdf:Property ;
    rdfs:label "variable" ;
    rdfs:comment "An IRI template variable" ;
    rdfs:domain hydra:IriTemplateMapping ;
    rdfs:isDefinedBy <http://www.w3.org/ns/hydra/core> ;
    rdfs:range xsd:string ;
    vs:term_status "testing" .

hydra:variableRepresentation a rdf:Property ;
    rdfs:label "variable representation" ;
    rdfs:comment "The representation format to use when expanding the IRI template." ;
    rdfs:domain hydra:IriTemplateMapping ;
    rdfs:isDefinedBy <http://www.w3.org/ns/hydra/core> ;
    rdfs:range hydra:VariableRepresentation ;
    vs:term_status "testing" .

hydra:view a hydra:Link ;
    rdfs:label "view" ;
    rdfs:comment "A specific view of a resource." ;
    rdfs:isDefinedBy <http://www.w3.org/ns/hydra/core> ;
    vs:term_status "testing" .

hydra:writeable rdfs:label "writable" ;
    rdfs:comment "This property is left for compatibility purposes and hydra:writable should be used instead." ;
    rdfs:isDefinedBy <http://www.w3.org/ns/hydra/core> ;
    rdfs:subPropertyOf hydra:writable ;
    vs:term_status "archaic" .

hydra:memberAssertion rdfs:label "member assertion" ;
    rdfs:comment "Semantics of each member provided by the collection." ;
    rdfs:domain hydra:Collection ;
    rdfs:isDefinedBy <http://www.w3.org/ns/hydra/core> ;
    vs:term_status "testing" .

hydra:pageReference a rdf:Property ;
    rdfs:label "page reference" ;
    rdfs:comment "Instructs to provide a specific page reference of the collection." ;
    rdfs:isDefinedBy <http://www.w3.org/ns/hydra/core> ;
    vs:term_status "testing" .

hydra:writable a rdf:Property ;
    rdfs:label "writable" ;
    rdfs:comment "True if the client can change the property's value, false otherwise." ;
    rdfs:domain hydra:SupportedProperty ;
    rdfs:isDefinedBy <http://www.w3.org/ns/hydra/core> ;
    rdfs:range xsd:boolean ;
    vs:term_status "testing" .

hydra:Rfc6570Template a rdfs:Datatype ;
    rdfs:label "RFC6570 IRI template" ;
    rdfs:comment "An IRI template as defined by RFC6570." ;
    rdfs:isDefinedBy <http://www.w3.org/ns/hydra/core> ;
    rdfs:range xsd:string ;
    rdfs:seeAlso <http://tools.ietf.org/html/rfc6570> ;
    vs:term_status "testing" .

hydra:BaseUriSource a hydra:Class ;
    rdfs:label "Base Uri source" ;
    rdfs:comment "Provides a base abstract for base Uri source for Iri template resolution." ;
    rdfs:isDefinedBy <http://www.w3.org/ns/hydra/core> ;
    rdfs:subClassOf hydra:Resource ;
    vs:term_status "testing" .

hydra:VariableRepresentation a hydra:Class ;
    rdfs:label "VariableRepresentation" ;
    rdfs:comment "A representation specifies how to serialize variable values into strings." ;
    rdfs:isDefinedBy <http://www.w3.org/ns/hydra/core> ;
    vs:term_status "testing" .

hydra:Collection a hydra:Class ;
    rdfs:label "Collection" ;
    rdfs:comment "A collection holding references to a number of related resources." ;
    rdfs:isDefinedBy <http://www.w3.org/ns/hydra/core> ;
    rdfs:subClassOf hydra:Resource ;
    vs:term_status "testing" .

hydra:IriTemplate a hydra:Class ;
    rdfs:label "IRI Template" ;
    rdfs:comment "The class of IRI templates." ;
    rdfs:isDefinedBy <http://www.w3.org/ns/hydra/core> ;
    vs:term_status "testing" .

hydra:TemplatedLink a hydra:Class ;
    rdfs:label "Templated Link" ;
    rdfs:comment "A templated link." ;
    rdfs:isDefinedBy <http://www.w3.org/ns/hydra/core> ;
    rdfs:subClassOf rdf:Property,
        hydra:Resource ;
    vs:term_status "testing" .

hydra:IriTemplateMapping a hydra:Class ;
    rdfs:label "IriTemplateMapping" ;
    rdfs:comment "A mapping from an IRI template variable to a property." ;
    rdfs:isDefinedBy <http://www.w3.org/ns/hydra/core> ;
    vs:term_status "testing" .

hydra:Status a hydra:Class ;
    rdfs:label "Status code description" ;
    rdfs:comment "Additional information about a status code that might be returned." ;
    rdfs:isDefinedBy <http://www.w3.org/ns/hydra/core> ;
    vs:term_status "testing" .

hydra:ApiDocumentation a hydra:Class ;
    rdfs:label "ApiDocumentation" ;
    rdfs:comment "The Hydra API documentation class" ;
    rdfs:isDefinedBy <http://www.w3.org/ns/hydra/core> ;
    rdfs:subClassOf hydra:Resource ;
    vs:term_status "testing" .

hydra:SupportedProperty a hydra:Class ;
    rdfs:label "Supported Property" ;
    rdfs:comment "A property known to be supported by a Hydra class." ;
    rdfs:isDefinedBy <http://www.w3.org/ns/hydra/core> ;
    vs:term_status "testing" .

hydra:Operation a hydra:Class ;
    rdfs:label "Operation" ;
    rdfs:comment "An operation." ;
    rdfs:isDefinedBy <http://www.w3.org/ns/hydra/core> ;
    vs:term_status "testing" .

hydra:Link a hydra:Class ;
    rdfs:label "Link" ;
    rdfs:comment "The class of properties representing links." ;
    rdfs:isDefinedBy <http://www.w3.org/ns/hydra/core> ;
    rdfs:subClassOf rdf:Property,
        hydra:Resource ;
    vs:term_status "testing" .

hydra:Resource a hydra:Class ;
    rdfs:label "Hydra Resource" ;
    rdfs:comment "The class of dereferenceable resources by means a client can attempt to dereference; however, the received responses should still be verified." ;
    rdfs:isDefinedBy <http://www.w3.org/ns/hydra/core> ;
    vs:term_status "testing" .

<http://www.w3.org/ns/hydra/core> a owl:Ontology ;
    rdfs:label "The Hydra Core Vocabulary" ;
    cc:attributionName "Hydra W3C Community Group" ;
    cc:attributionURL <http://www.hydra-cg.com/> ;
    cc:license <http://creativecommons.org/licenses/by/4.0/> ;
    dc:description "The Hydra Core Vocabulary is a lightweight vocabulary to create hypermedia-driven Web APIs. By specifying a number of concepts commonly used in Web APIs it enables the creation of generic API clients." ;
    dc:publisher "Hydra W3C Community Group" ;
    dc:rights "Copyright © 2012-2014 the Contributors to the Hydra Core Vocabulary Specification" ;
    vann:preferredNamespacePrefix "hydra" ;
    rdfs:comment "A lightweight vocabulary for hypermedia-driven Web APIs" ;
    rdfs:seeAlso <https://www.hydra-cg.com/spec/latest/core/> .
